Types based upon finite maps encode correctly and simple functions from the opsem script translate. Some of the script has been translated in fmapExample.sml, however, translations now require conditional translation on successful evalation.

examples/acl2/examples/fmapExample.sml
@@ -1,11 +1,232 @@
 (*****************************************************************************)
 (* Test script for encoding using finite maps.                               *)
+(* This is based on the opsem script with translations placed after each     *)
+(* definition to mark progress.                                              *)
 (*****************************************************************************)
 
-load "acl2encodeLib";
+set_trace "Unicode" 0;
+set_trace "pp_annotations" 0;
 
-val tf_def = Define `tf (x : int |-> int) = if 0 IN FDOM x then x ' 0 else 0`;
+app load ["acl2encodeLib", "stringLib", "finite_mapTheory", "intLib",
+          "pred_setTheory","whileTheory","optionTheory","unwindLib", "finite_mapTheory"];
+open HolKernel Parse boolLib bossLib
+     stringLib IndDefLib IndDefRules finite_mapTheory relationTheory
+     arithmeticTheory prim_recTheory
+     pred_setTheory whileTheory combinTheory optionTheory unwindLib;
+intLib.deprecate_int();
+clear_overloads_on "TC"; (* Stop TC R printing as TC^+ *)
+
+
+val _ =
+ Hol_datatype
+  `value = Scalar of int | Array  of (num |-> int)`;
+
+val _ = acl2encodeLib.initialise_type ``:value``;
+
+val _ = type_abbrev("state", ``:string |-> value``);
+val _ = type_abbrev("sfun",  ``:state  ->  state``);
+val _ = type_abbrev("pred",  ``:state  ->  bool``);
+val _ = type_abbrev("vars",  ``:string ->  bool``);
+
+val isScalar_def =
+ Define
+  `(isScalar(Scalar n) = T) /\ (isScalar(Array a) = F)`;
+
+val _ = acl2encodeLib.translate_simple_function [(``isScalar``, "acl2isScalar")] isScalar_def;
+
+val ScalarOf_def =
+ Define
+  `ScalarOf(Scalar n) = n`;
+
+val _ = acl2encodeLib.translate_simple_function [(``ScalarOf``, "acl2ScalarOf")] ScalarOf_def;
+
+val isArray_def =
+ Define
+  `(isArray(Array a) = T) /\ (isArray(Scalar n) = F)`;
+
+val _ = acl2encodeLib.translate_simple_function [(``isArray``, "acl2isArray")] isArray_def;
+
+val ArrayOf_def =
+ Define
+  `ArrayOf(Array a) = a`;
+
+val _ = encodeLib.set_bottom_value ``:num |-> int`` ``FEMPTY : num |-> int``;
+
+val _ = acl2encodeLib.translate_simple_function [(``ArrayOf``, "acl2ArrayOf")] ArrayOf_def;
+
+(*---------------------------------------------------------------------------*)
+(* Syntax of the programming language.					     *)
+(*---------------------------------------------------------------------------*)
+
+(*---------------------------------------------------------------------------*)
+(* Natural number (nexp), boolean (bexp) and array expressions (aexp)        *)
+(* are defined by datatypes with simple evaluation semantics.                *)
+(*---------------------------------------------------------------------------*)
+
+val _ =
+ Hol_datatype
+  `nexp = Var of string
+        | Arr of string => nexp
+        | Const of int
+        | Plus of nexp => nexp
+        | Sub of nexp => nexp
+        | Times of nexp => nexp
+        | Div of nexp => nexp
+        | Min of nexp => nexp`;
+
+val _ = acl2encodeLib.initialise_type ``:nexp``;
+
+val _ =
+ Hol_datatype
+  `bexp = Equal of nexp => nexp
+        | Less of nexp => nexp
+        | LessEq of nexp => nexp
+        | Greater of nexp => nexp
+        | GreaterEq of nexp => nexp
+        | And of bexp => bexp
+        | Or of bexp => bexp
+        | Not of bexp`;
+
+val _ = acl2encodeLib.initialise_type ``:bexp``;
+
+
+val neval_def =
+ Define
+  `(neval (Var v) s = ScalarOf(s ' v)) /\
+   (neval (Arr a e) s = (ArrayOf(s ' a) ' (Num(neval e s)))) /\
+   (neval (Const c) s = c) /\
+   (neval (Plus e1 e2) s = integer$int_add (neval e1 s) (neval e2 s)) /\
+   (neval (Sub e1 e2) s = integer$int_sub (neval e1 s) (neval e2 s)) /\
+   (neval (Times e1 e2) s = integer$int_mul (neval e1 s) (neval e2 s)) /\
+   (neval (Div e1 e2) s = integer$int_quot (neval e1 s) (neval e2 s)) /\
+   (neval (Min e1 e2) s = integer$int_min (neval e1 s) (neval e2 s))`;
+
+(*****************************************************************************)
+(* neval is not a complete function. It cannot complete if any variable in   *)
+(* the expression is not in the environment. Therefore, we must define an    *)
+(* auxilliary function to determine when a call to neval is safe             *)
+(*                                                                           *)
+(* Unfortunately, this will rely on neval to determine array indices.        *)
+(* To avoid a mutually recurse translation we define 'safe_neval' that acts  *)
+(* as 'neval' but returns 0 where 'neval' would stop evaluating.             *)
+(*****************************************************************************)
+
+val safe_neval_def = 
+  Define 
+  `(safe_neval (Var v) s = if v IN FDOM s /\ isScalar (s ' v) then ScalarOf(s ' v) else 0i) /\
+   (safe_neval (Arr a e) s = if a IN FDOM s /\ isArray (s ' a) /\ integer$int_le 0i (safe_neval e s) /\ Num (safe_neval e s) IN FDOM (ArrayOf (s ' a)) then (ArrayOf(s ' a) ' (Num(safe_neval e s))) else 0i) /\
+   (safe_neval (Const c) s = c) /\
+   (safe_neval (Plus e1 e2) s = integer$int_add (safe_neval e1 s) (safe_neval e2 s)) /\
+   (safe_neval (Sub e1 e2) s = integer$int_sub (safe_neval e1 s) (safe_neval e2 s)) /\
+   (safe_neval (Times e1 e2) s = integer$int_mul (safe_neval e1 s) (safe_neval e2 s)) /\
+   (safe_neval (Div e1 e2) s = if safe_neval e2 s = 0i then 0i else integer$int_quot (safe_neval e1 s) (safe_neval e2 s)) /\
+   (safe_neval (Min e1 e2) s = integer$int_min (safe_neval e1 s) (safe_neval e2 s))`;
+
+(*****************************************************************************)
+(* We can then use this to define nevaluates as follows:                     *)
+(*****************************************************************************)
+
+val nevaluates_def = 
+  Define `(nevaluates (Var v) s = v IN FDOM s /\ isScalar (s ' v)) /\
+          (nevaluates (Arr a e) s = a IN FDOM s /\ isArray (s ' a) /\ integer$int_le 0i (safe_neval e s) /\ nevaluates e s /\ Num (safe_neval e s) IN FDOM (ArrayOf (s ' a))) /\
+	  (nevaluates (Const c) s = T) /\
+	  (nevaluates (Plus e1 e2) s = nevaluates e1 s /\ nevaluates e2 s) /\
+	  (nevaluates (Sub e1 e2) s = nevaluates e1 s /\ nevaluates e2 s) /\
+	  (nevaluates (Times e1 e2) s = nevaluates e1 s /\ nevaluates e2 s) /\
+	  (nevaluates (Div e1 e2) s = ~(safe_neval e2 s = 0i) /\ nevaluates e1 s /\ nevaluates e2 s) /\
+	  (nevaluates (Min e1 e2) s = nevaluates e1 s /\ nevaluates e2 s)`;
+
+(*****************************************************************************)
+(* ...and prove that this implies we are correct.                            *)
+(*****************************************************************************)
+
+val neval_safe_theorem1 = store_thm("neval_safe_theorem1",
+    ``!e s. nevaluates e s ==> (safe_neval e s = neval e s)``,
+    Induct THEN RW_TAC std_ss [nevaluates_def, safe_neval_def, neval_def]);
+
+(*****************************************************************************)
+(* We now begin by translating safe_neval.                                   *)
+(*****************************************************************************)
+
+val ONE_ONE_str = prove(``ONE_ONE str``, RW_TAC std_ss [ONE_ONE_THM]);
+val ONE_ONE_nat = prove(``ONE_ONE nat``, RW_TAC std_ss [ONE_ONE_THM, sexpTheory.nat_def, translateTheory.INT_CONG, integerTheory.INT_INJ]);
+
+val _ = acl2encodeLib.translate_conditional_function [(``safe_neval``,"acl2safe_neval")] [ONE_ONE_str, ONE_ONE_nat] safe_neval_def;
+
+val _ = acl2encodeLib.translate_conditional_function [(``nevaluates``,"acl2nevaluates")] [ONE_ONE_str, ONE_ONE_nat] nevaluates_def;
+
+(*****************************************************************************)
+(* The next stage is to translate neval as a 'limit' function using          *)
+(* nevaluates as the limit.                                                  *)
+(*****************************************************************************)
+
+(*
+
+val _ =
+ Hol_datatype
+  `aexp = ArrConst  of (num |-> int)           (* array constant *)
+        | ArrVar    of string                  (* array variable *)
+        | ArrUpdate of aexp => nexp => nexp`;  (* array update   *)
+
+val _ = acl2encodeLib.initialise_type ``:aexp``;
+
+val beval_def =
+ Define
+  `(beval (Equal e1 e2) s = (neval e1 s = neval e2 s)) /\
+   (beval (Less e1 e2) s = integer$int_lt (neval e1 s) (neval e2 s)) /\
+   (beval (LessEq e1 e2) s = integer$int_le (neval e1 s) (neval e2 s)) /\
+   (beval (Greater e1 e2) s = integer$int_gt (neval e1 s) (neval e2 s)) /\
+   (beval (GreaterEq e1 e2) s = integer$int_ge (neval e1 s) (neval e2 s)) /\
+   (beval (And b1 b2) s = (beval b1 s /\ beval b2 s)) /\
+   (beval (Or b1 b2) s = (beval b1 s \/ beval b2 s)) /\
+   (beval (Not e) s = ~(beval e s))`;
+
+val aeval_def =
+ Define
+  `(aeval (ArrConst f) s = f)
+   /\
+   (aeval (ArrVar v) s = ArrayOf(s ' v))
+   /\
+   (aeval (ArrUpdate a e1 e2) s = aeval a s |+ (Num(neval e1 s), neval e2 s))`;
+
+val naeval_def =
+ Define
+  `(naeval (INL e) s = Scalar(neval e s))
+   /\
+   (naeval (INR a) s = Array(aeval a s))`;
+
+val Update_def =
+ Define
+  `Update v e s = s |+ (v, naeval e s)`;
+
+val UpdateCases =
+ store_thm
+  ("UpdateCases",
+   ``(Update v (INL e) s = s |+ (v, Scalar(neval e s)))
+     /\
+     (Update v (INR a) s = s |+ (v, Array(aeval a s)))``,
+   RW_TAC std_ss [Update_def,naeval_def]);
+
+(* Convert a value or array to a constant expression *)
+val Exp_def =
+ Define
+  `(Exp(Scalar n) = INL(Const n))
+   /\
+   (Exp(Array f)  = INR(ArrConst f))`;
+
+val Update_Exp =
+ store_thm
+  ("Update_Exp",
+   ``!v val s. Update v (Exp val) s = s |+ (v, val)``,
+   Cases_on `val`
+    THEN RW_TAC std_ss [UpdateCases,Exp_def,aeval_def,neval_def]);
+
+val _ = acl2encodeLib.translate_conditional_function [(``neval``, "acl2neval")] [] neval_def;
+
+
+val tf_def = Define `tf (x : int |-> int) = if 0i IN FDOM x then x ' 0i else 0i`;
 
 val oneone_int = ONEONE_ENC_THM ``:int``;
 
 val _ = acl2encodeLib.translate_conditional_function [(``tf``, "test_tf")] [oneone_int] tf_def handle e => acl2encodeLib.Raise e;
+*)
